src/cddl/pulse/CDDL.Pulse.Serialize.ArrayGroup.fst
@@ -1,0 +1,264 @@
+module CDDL.Pulse.Serialize.ArrayGroup
+#lang-pulse
+
+inline_for_extraction noextract [@@noextract_to "krml"]
+fn impl_serialize_array
+   (cbor_det_serialize_array: cbor_det_serialize_array_t)
+    (# [@@@erasable] t: Ghost.erased (array_group None))
+    (# [@@@erasable] tgt: Type0)
+    (# [@@@erasable] inj: Ghost.erased bool)
+    (# [@@@erasable] s: Ghost.erased (ag_spec t tgt inj))
+    (#impl_tgt: Type0)
+    (# [@@@erasable] r: rel impl_tgt tgt)
+    (i: impl_serialize_array_group s r)
+: impl_serialize #_ #_ #_ (spec_array_group s) #_ r
+=
+  (c: _)
+  (#v: _)
+  (out: _)
+{
+  let mut pcount = 0uL;
+  let mut psize = 0sz;
+  Cbor.cbor_det_serialize_list_nil ();
+  let res = i c out pcount psize [];
+  Classical.forall_intro (Classical.move_requires Cbor.cbor_det_serialize_array_length_gt_list);
+  if (res) {
+    let size = !psize;
+    let count = !pcount;
+    cbor_det_serialize_array count out (s.ag_serializer v) size
+  } else {
+    0sz
+  }
+}
+
+inline_for_extraction noextract [@@noextract_to "krml"]
+fn impl_serialize_array_group_ext
+    (#[@@@erasable]t: Ghost.erased (array_group None))
+    (#[@@@erasable]tgt: Type0)
+    (#[@@@erasable] inj: Ghost.erased bool)
+    (#[@@@erasable]ps: Ghost.erased (ag_spec t tgt inj))
+    (#impl_tgt: Type0)
+    (#[@@@erasable]r: rel impl_tgt tgt)
+    (i: impl_serialize_array_group ps r)
+    (#[@@@erasable]t': Ghost.erased (array_group None))
+    (#[@@@erasable] inj': Ghost.erased bool)
+    ([@@@erasable]ps': Ghost.erased (ag_spec t' tgt inj'))
+    ([@@@erasable]sq: squash (
+      (Ghost.reveal inj == true \/ Ghost.reveal inj' == true) /\
+      array_group_equiv t' t /\
+      (forall (x: list cbor) . array_group_parser_spec_refinement (Ghost.reveal t') x ==> ((Ghost.reveal ps'.ag_parser x <: tgt) == Ghost.reveal ps.ag_parser x))
+    ))
+: impl_serialize_array_group #(Ghost.reveal t') #tgt #inj' (Ghost.reveal ps') #impl_tgt r
+=
+    (c: _)
+    (#v: _)
+    (out: _)
+    (out_count: _)
+    (out_size: _)
+    (l: _)
+{
+  i c out out_count out_size l
+}
+
+inline_for_extraction noextract [@@noextract_to "krml";
+  FStar.Tactics.postprocess_with (fun _ -> FStar.Tactics.norm [delta; zeta; iota; primops]; FStar.Tactics.trefl ())
+]
+let pow2_64_m1 : U64.t = U64.uint_to_t (pow2 64 - 1)
+
+let pow2_64_m1_eq : squash (U64.v pow2_64_m1 == pow2 64 - 1) = _ by (
+  FStar.Tactics.norm [delta; zeta; iota; primops];
+  FStar.Tactics.trefl ()
+)
+
+let list_append_length_pat
+  (#t: Type)
+  (l1 l2: list t)
+: Lemma
+  (List.Tot.length (List.Tot.append l1 l2) == List.Tot.length l1 + List.Tot.length l2)
+  [SMTPat (List.Tot.append l1 l2)]
+= List.Tot.append_length l1 l2
+
+let impl_serialize_array_group_item_correct
+    (#t: typ)
+    (#tgt: Type0)
+    (#inj: bool)
+    (ps: spec t tgt inj)
+    (l: list Cbor.cbor)
+    (v: tgt)
+    (size': nat)
+: Lemma
+  ((
+    ps.serializable v /\
+    Seq.length (Cbor.cbor_det_serialize (ps.serializer v)) <= size'
+  ) <==> (
+    (ag_spec_item ps).ag_serializable v /\
+    Seq.length (Cbor.cbor_det_serialize_list (List.Tot.append l ((ag_spec_item ps).ag_serializer v))) <= Seq.length (Cbor.cbor_det_serialize_list l) + size'
+  ))
+= assert (ps.serializable v == (ag_spec_item ps).ag_serializable v);
+  if (ps.serializable v)
+  then begin
+    Cbor.cbor_det_serialize_list_snoc l (ps.serializer v)
+  end
+
+let seq_slice_append
+  (#t: Type)
+  (s1 s2: Seq.seq t)
+: Lemma
+  (ensures
+    Seq.slice (Seq.append s1 s2) 0 (Seq.length s1) `Seq.equal` s1 /\
+    Seq.slice (Seq.append s1 s2) (Seq.length s1) (Seq.length s1 + Seq.length s2) `Seq.equal` s2
+  )
+= ()
+
+inline_for_extraction noextract [@@noextract_to "krml"]
+fn impl_serialize_array_group_item
+    (#[@@@erasable]t: Ghost.erased typ)
+    (#[@@@erasable]tgt: Type0)
+    (#[@@@erasable]inj: Ghost.erased bool)
+    (#[@@@erasable]ps: Ghost.erased (spec t tgt inj))
+    (#impl_tgt: Type0)
+    (#[@@@erasable]r: rel impl_tgt tgt)
+    (i: impl_serialize ps r)
+: impl_serialize_array_group #_ #_ #_ (ag_spec_item ps) #_ r
+= 
+    (c: _)
+    (#v: _)
+    (out: _)
+    (out_count: _)
+    (out_size: _)
+    (l: _)
+{
+  let count = !out_count;
+  if (U64.lt count pow2_64_m1) {
+    let size = !out_size;
+    with w . assert (pts_to out w);
+    Seq.lemma_split w (SZ.v size);
+    let (out0, out1) = S.split out size;
+    let w0 = Ghost.hide (Cbor.cbor_det_serialize_list l);
+    assert (pts_to out0 w0);
+    let size1 = i c out1;
+    S.pts_to_len out1;
+    with w1 . assert (pts_to out1 w1);
+    seq_slice_append w0 w1;
+    S.join _ _ out;
+    S.pts_to_len out;
+    impl_serialize_array_group_item_correct ps l v (SZ.v (S.len out1));
+    if (size1 = 0sz) {
+      false
+    } else {
+      Cbor.cbor_det_serialize_list_snoc l (ps.serializer v);
+      out_count := U64.add count 1uL;
+      out_size := (SZ.add size size1);
+      true
+    }
+  } else {
+    false
+  }
+}
+
+let list_append_assoc_pat
+  (#t: Type)
+  (l1 l2 l3: list t)
+: Lemma
+  (ensures (List.Tot.append l1 (List.Tot.append l2 l3) == List.Tot.append (List.Tot.append l1 l2) l3))
+  [SMTPatOr [
+    [SMTPat (List.Tot.append l1 (List.Tot.append l2 l3))];
+    [SMTPat (List.Tot.append (List.Tot.append l1 l2) l3)];
+  ]]
+= List.Tot.append_assoc l1 l2 l3
+
+let cbor_det_serialize_list_append_pat
+  (l1 l2: list cbor)
+: Lemma
+  (ensures (Cbor.cbor_det_serialize_list (List.Tot.append l1 l2) == Seq.append (Cbor.cbor_det_serialize_list l1) (Cbor.cbor_det_serialize_list l2)))
+  [SMTPat (Cbor.cbor_det_serialize_list (List.Tot.append l1 l2))]
+= Cbor.cbor_det_serialize_list_append l1 l2
+
+inline_for_extraction noextract [@@noextract_to "krml"]
+fn impl_serialize_array_group_concat
+    (#[@@@erasable]t1: Ghost.erased (array_group None))
+    (#[@@@erasable]tgt1: Type0)
+    (#[@@@erasable] inj1: Ghost.erased bool)
+    (#[@@@erasable]ps1: Ghost.erased (ag_spec t1 tgt1 inj1))
+    (#impl_tgt1: Type0)
+    (#[@@@erasable]r1: rel impl_tgt1 tgt1)
+    (i1: impl_serialize_array_group ps1 r1)
+    (#[@@@erasable]t2: Ghost.erased (array_group None))
+    (#[@@@erasable]tgt2: Type0)
+    (#[@@@erasable] inj2: Ghost.erased bool)
+    (#[@@@erasable]ps2: Ghost.erased (ag_spec t2 tgt2 inj2))
+    (#impl_tgt2: Type0)
+    (#[@@@erasable]r2: rel impl_tgt2 tgt2)
+    (i2: impl_serialize_array_group ps2 r2)
+    (sq: squash (
+      array_group_concat_unique_weak t1 t2
+    ))
+: impl_serialize_array_group #_ #_ #_ (ag_spec_concat ps1 ps2) #_ (rel_pair r1 r2)
+=
+    (c: _)
+    (#v: _)
+    (out: _)
+    (out_count: _)
+    (out_size: _)
+    (l: _)
+{
+  norewrite let (c1, c2) = c;
+  Trade.rewrite_with_trade (rel_pair r1 r2 c v) (r1 c1 (fst v) ** r2 c2 (snd v));
+  let res1 = i1 c1 out out_count out_size l;
+  S.pts_to_len out;
+  if (res1) {
+    let res2 = i2 c2 out out_count out_size (List.Tot.append l (ps1.ag_serializer (fst v)));
+    Trade.elim _ _;
+    res2
+  } else {
+    Trade.elim _ _;
+    false
+  }
+}
+
+inline_for_extraction noextract [@@noextract_to "krml"]
+fn impl_serialize_array_group_choice
+    (#[@@@erasable]t1: Ghost.erased (array_group None))
+    (#[@@@erasable]tgt1: Type0)
+    (#[@@@erasable] inj1: Ghost.erased bool)
+    (#[@@@erasable]ps1: Ghost.erased (ag_spec t1 tgt1 inj1))
+    (#impl_tgt1: Type0)
+    (#[@@@erasable]r1: rel impl_tgt1 tgt1)
+    (i1: impl_serialize_array_group ps1 r1)
+    (#[@@@erasable]t2: Ghost.erased (array_group None))
+    (#[@@@erasable]tgt2: Type0)
+    (#[@@@erasable] inj2: Ghost.erased bool)
+    (#[@@@erasable]ps2: Ghost.erased (ag_spec t2 tgt2 inj2))
+    (#impl_tgt2: Type0)
+    (#[@@@erasable]r2: rel impl_tgt2 tgt2)
+    (i2: impl_serialize_array_group ps2 r2)
+    (sq: squash (
+      array_group_disjoint t1 t2
+    ))
+: impl_serialize_array_group #_ #_ #_ (ag_spec_choice ps1 ps2) #_ (rel_either r1 r2)
+=
+    (c: _)
+    (#v: _)
+    (out: _)
+    (out_count: _)
+    (out_size: _)
+    (l: _)
+{
+  rel_either_cases r1 r2 c v;
+  match c {
+    norewrite
+    Inl c1 -> {
+      Trade.rewrite_with_trade (rel_either r1 r2 c v) (r1 c1 (Inl?.v v));
+      let res = i1 c1 out out_count out_size l;
+      Trade.elim _ _;
+      res
+    }
+    norewrite
+    Inr c2 -> {
+      Trade.rewrite_with_trade (rel_either r1 r2 c v) (r2 c2 (Inr?.v v));
+      let res = i2 c2 out out_count out_size l;
+      Trade.elim _ _;
+      res
+    }
+  }
+}
