src/cddl/pulse/CDDL.Pulse.Serialize.ArrayGroup.fsti
@@ -1,0 +1,130 @@
+module CDDL.Pulse.Serialize.ArrayGroup
+include CDDL.Pulse.Serialize.Base
+include CDDL.Pulse.Parse.ArrayGroup
+open Pulse.Lib.Pervasives
+open CBOR.Spec.API.Type
+open CBOR.Pulse.API.Base
+module Trade = Pulse.Lib.Trade.Util
+module R = Pulse.Lib.Reference
+module S = Pulse.Lib.Slice
+module U8 = FStar.UInt8
+module SZ = FStar.SizeT
+module Cbor = CBOR.Spec.API.Format
+module U64 = FStar.UInt64
+
+let impl_serialize_array_group_pre
+  (count: U64.t)
+  (size: SZ.t)
+  (l: list Cbor.cbor)
+  (w: Seq.seq U8.t)
+: Tot prop
+= List.Tot.length l == U64.v count /\
+  SZ.v size <= Seq.length w /\
+  Seq.slice w 0 (SZ.v size) `Seq.equal` Cbor.cbor_det_serialize_list l
+
+let impl_serialize_array_group_post
+  (count: U64.t)
+  (size: SZ.t)
+  (l: list Cbor.cbor)
+  (#t: array_group None)
+  (#tgt: Type0)
+  (#inj: bool)
+  (s: ag_spec t tgt inj)
+  (v: tgt)
+  (w: Seq.seq U8.t)
+  (res: bool)
+: Tot prop
+= (res == true <==> (
+    s.ag_serializable v /\
+    FStar.UInt.fits (List.Tot.length l + List.Tot.length (s.ag_serializer v)) 64 /\
+    Seq.length (Cbor.cbor_det_serialize_list (List.Tot.append l (s.ag_serializer v))) <= Seq.length w
+  )) /\
+  (res == true ==> (
+    impl_serialize_array_group_pre count size (List.Tot.append l (s.ag_serializer v)) w
+  ))
+
+inline_for_extraction noextract [@@noextract_to "krml"]
+let impl_serialize_array_group
+    (#t: array_group None)
+    (#tgt: Type0)
+    (#inj: bool)
+    (s: ag_spec t tgt inj)
+    (#impl_tgt: Type0)
+    (r: rel impl_tgt tgt)
+=
+  (c: impl_tgt) ->
+  (#v: Ghost.erased tgt) ->
+  (out: S.slice U8.t) ->
+  (out_count: R.ref U64.t) ->
+  (out_size: R.ref SZ.t) ->
+  (l: Ghost.erased (list Cbor.cbor)) ->
+  stt bool
+    (exists* w count size . r c v ** pts_to out w ** pts_to out_count count ** pts_to out_size size **
+      pure (impl_serialize_array_group_pre count size l w)
+    )
+    (fun res -> exists* w count' size' . r c v ** pts_to out w ** pts_to out_count count' ** pts_to out_size size' ** pure (
+      impl_serialize_array_group_post count' size' l s v w res
+    ))
+
+inline_for_extraction noextract [@@noextract_to "krml"]
+val impl_serialize_array
+   (cbor_det_serialize_array: cbor_det_serialize_array_t)
+    (# [@@@erasable] t: Ghost.erased (array_group None))
+    (# [@@@erasable] tgt: Type0)
+    (# [@@@erasable] inj: Ghost.erased bool)
+    (# [@@@erasable] s: Ghost.erased (ag_spec t tgt inj))
+    (#impl_tgt: Type0)
+    (# [@@@erasable] r: rel impl_tgt tgt)
+    (i: impl_serialize_array_group s r)
+: impl_serialize #_ #_ #_ (spec_array_group s) #_ r
+
+inline_for_extraction noextract [@@noextract_to "krml"]
+val impl_serialize_array_group_ext
+    (#[@@@erasable]t: Ghost.erased (array_group None))
+    (#[@@@erasable]tgt: Type0)
+    (#[@@@erasable] inj: Ghost.erased bool)
+    (#[@@@erasable]ps: Ghost.erased (ag_spec t tgt inj))
+    (#impl_tgt: Type0)
+    (#[@@@erasable]r: rel impl_tgt tgt)
+    (i: impl_serialize_array_group ps r)
+    (#[@@@erasable]t': Ghost.erased (array_group None))
+    (#[@@@erasable] inj': Ghost.erased bool)
+    ([@@@erasable]ps': Ghost.erased (ag_spec t' tgt inj'))
+    ([@@@erasable]sq: squash (
+      (Ghost.reveal inj == true \/ Ghost.reveal inj' == true) /\
+      array_group_equiv t' t /\
+      (forall (x: list cbor) . array_group_parser_spec_refinement (Ghost.reveal t') x ==> ((ps'.ag_parser x <: tgt) == ps.ag_parser x))
+    ))
+: impl_serialize_array_group #(Ghost.reveal t') #tgt #inj' (Ghost.reveal ps') #impl_tgt r
+
+inline_for_extraction noextract [@@noextract_to "krml"]
+val impl_serialize_array_group_item
+    (#[@@@erasable]t: Ghost.erased typ)
+    (#[@@@erasable]tgt: Type0)
+    (#[@@@erasable]inj: Ghost.erased bool)
+    (#[@@@erasable]ps: Ghost.erased (spec t tgt inj))
+    (#impl_tgt: Type0)
+    (#[@@@erasable]r: rel impl_tgt tgt)
+    (i: impl_serialize ps r)
+: impl_serialize_array_group #_ #_ #_ (ag_spec_item ps) #_ r
+
+inline_for_extraction noextract [@@noextract_to "krml"]
+val impl_serialize_array_group_concat
+    (#[@@@erasable]t1: Ghost.erased (array_group None))
+    (#[@@@erasable]tgt1: Type0)
+    (#[@@@erasable] inj1: Ghost.erased bool)
+    (#[@@@erasable]ps1: Ghost.erased (ag_spec t1 tgt1 inj1))
+    (#impl_tgt1: Type0)
+    (#[@@@erasable]r1: rel impl_tgt1 tgt1)
+    (i1: impl_serialize_array_group ps1 r1)
+    (#[@@@erasable]t2: Ghost.erased (array_group None))
+    (#[@@@erasable]tgt2: Type0)
+    (#[@@@erasable] inj2: Ghost.erased bool)
+    (#[@@@erasable]ps2: Ghost.erased (ag_spec t2 tgt2 inj2))
+    (#impl_tgt2: Type0)
+    (#[@@@erasable]r2: rel impl_tgt2 tgt2)
+    (i2: impl_serialize_array_group ps2 r2)
+    (sq: squash (
+      array_group_concat_unique_weak t1 t2
+    ))
+: impl_serialize_array_group #_ #_ #_ (ag_spec_concat ps1 ps2) #_ (rel_pair r1 r2)
