src/cddl/pulse/CDDL.Pulse.Serialize.Base.fst
@@ -1,0 +1,133 @@
+module CDDL.Pulse.Serialize.Base
+#lang-pulse
+include CDDL.Pulse.Base
+include CDDL.Pulse.Types
+open Pulse.Lib.Pervasives
+open CBOR.Spec.API.Type
+open CBOR.Pulse.API.Base
+module Trade = Pulse.Lib.Trade.Util
+module S = Pulse.Lib.Slice
+module U8 = FStar.UInt8
+module SZ = FStar.SizeT
+module Cbor = CBOR.Spec.API.Format
+
+let impl_serialize_post
+    (#t: typ)
+    (#tgt: Type0)
+    (#inj: bool)
+    (s: spec t tgt inj)
+    (v: tgt)
+    (w: Seq.seq U8.t)
+    (res: SZ.t)
+: Tot prop
+= (SZ.v res > 0 <==> (s.serializable v /\ Seq.length (Cbor.cbor_det_serialize (s.serializer v)) <= Seq.length w)) /\
+  (SZ.v res > 0 ==> (
+    SZ.v res <= Seq.length w /\
+    Seq.slice w 0 (SZ.v res) == Cbor.cbor_det_serialize (s.serializer v)
+  ))
+
+inline_for_extraction noextract [@@noextract_to "krml"]
+let impl_serialize
+    (#t: typ)
+    (#tgt: Type0)
+    (#inj: bool)
+    (s: spec t tgt inj)
+    (#impl_tgt: Type0)
+    (r: rel impl_tgt tgt)
+=
+  (c: impl_tgt) ->
+  (#v: Ghost.erased tgt) ->
+  (out: S.slice U8.t) ->
+  stt SZ.t
+    (exists* w . r c v ** pts_to out w)
+    (fun res -> exists* w .
+      r c v ** pts_to out w **
+      pure (impl_serialize_post s v w res)
+    )
+
+inline_for_extraction noextract [@@noextract_to "krml"]
+fn impl_serialize_always_false
+    (#t: Ghost.erased typ)
+    (#inj: Ghost.erased bool)
+    (s: Ghost.erased (spec t (squash False) inj))
+: impl_serialize #_ #_ #_ s #_ (rel_always_false (squash False) (squash False))
+= (c: _)
+  (#v: _)
+  (out: _)
+{
+  0sz
+}
+
+inline_for_extraction noextract [@@noextract_to "krml"]
+fn impl_serialize_ext
+    (#[@@@erasable]t: Ghost.erased typ)
+    (#[@@@erasable]tgt: Type0)
+    (#[@@@erasable] inj: Ghost.erased bool)
+    (#[@@@erasable]ps: Ghost.erased (spec t tgt inj))
+    (#impl_tgt: Type0)
+    (#[@@@erasable]r: rel impl_tgt tgt)
+    (i: impl_serialize ps r)
+    (#[@@@erasable]t': Ghost.erased typ)
+    (#[@@@erasable] inj': Ghost.erased bool)
+    ([@@@erasable]ps': Ghost.erased (spec t' tgt inj'))
+    ([@@@erasable]sq: squash (
+      (Ghost.reveal inj == true \/ Ghost.reveal inj' == true) /\
+      typ_equiv t' t /\
+      (forall (x: cbor) . Ghost.reveal t' x ==> ((Ghost.reveal ps'.parser x <: tgt) == Ghost.reveal ps.parser x))
+    ))
+: impl_serialize #(Ghost.reveal t') #tgt #inj' (Ghost.reveal ps') #impl_tgt r
+=
+    (c: _)
+    (#v: _)
+    (out: _)
+{
+  i c out
+}
+
+inline_for_extraction noextract [@@noextract_to "krml"]
+fn impl_serialize_choice
+    (#[@@@erasable]t1: Ghost.erased typ)
+    (#[@@@erasable]tgt1: Type0)
+    (#[@@@erasable] inj1: Ghost.erased bool)
+    (#[@@@erasable]ps1: Ghost.erased (spec t1 tgt1 inj1))
+    (#impl_tgt1: Type0)
+    (#[@@@erasable]r1: rel impl_tgt1 tgt1)
+    (i1: impl_serialize ps1 r1)
+    (#[@@@erasable]t2: Ghost.erased typ)
+    (#[@@@erasable]tgt2: Type0)
+    (#[@@@erasable] inj2: Ghost.erased bool)
+    (#[@@@erasable]ps2: Ghost.erased (spec t2 tgt2 inj2))
+    (#impl_tgt2: Type0)
+    (#[@@@erasable]r2: rel impl_tgt2 tgt2)
+    (i2: impl_serialize ps2 r2)
+    ([@@@erasable]sq: squash (
+      typ_disjoint t1 t2
+    ))
+: impl_serialize #_ #_ #_ (spec_choice ps1 ps2) #_ (rel_either r1 r2)
+=
+    (c: _)
+    (#v: _)
+    (out: _)
+{
+  rel_either_cases r1 r2 c v;
+  match c {
+    norewrite
+    Inl c1 -> {
+      Trade.rewrite_with_trade
+        (rel_either r1 r2 c v)
+        (r1 c1 (Inl?.v v));
+      let res = i1 c1 out;
+      Trade.elim _ _;
+      res
+    }
+    norewrite
+    Inr c2 -> {
+      Trade.rewrite_with_trade
+        (rel_either r1 r2 c v)
+        (r2 c2 (Inr?.v v));
+      let res = i2 c2 out;
+      Trade.elim _ _;
+      res
+    }
+  }
+}
